# Classes for CONTENTdm metadata

@prefix cdmc: <http://doiTbdForThisDocument/> .
@prefix rdf: <http://www.w3.org/1999/02/22-rdf-syntax-ns#> .
@prefix rdfs:  <http://www.w3.org/2000/01/rdf-schema#> .
@prefix edm: <http://www.europeana.eu/schemas/edm/> .
@prefix dpla: <http://dp.la/about/map/> .
@prefix dct: <http://purl.org/dc/terms/> .

# Classes:
# cdmc:OrderNumber
# cdmc:NegativeNumber
# cdmc:PhotographersReferenceNumber

cdmc:OrderNumber a rdfs:Class ;
  rdfs:isDefinedBy <http://doiTbdForThisDocument/> ;
  rdfs:subClassOf rdfs:Literal ;
  rdfs:label "Order Number" ;
  dct:description "An order number for the item to be used when contacting the University of Washington Libraries Special Collections Reproduction Services." ;
  rdfs:seeAlso <https://github.com/UniverityOfWashingtonLibrariesSchemas/schemasProject/blob/master/dataDictionaries/html/ayp-horizontal-staff.html> .

cdmc:NegativeNumber a rdfs:Class ;
  rdfs:isDefinedBy <http://doiTbdForThisDocument/> ;
  rdfs:subClassOf rdfs:Literal ;
  rdfs:label "Negative Number" ;
  dct:description "An identifier used by the University of Washington Libraries Special Collections to track a photographic negative or negatives associated with an image." ;
  rdfs:seeAlso <https://github.com/UniverityOfWashingtonLibrariesSchemas/schemasProject/blob/master/dataDictionaries/html/ayp-horizontal-staff.html> .

cdmc:PhotographersReferenceNumber a rdfs:Class ;
  rdfs:isDefinedBy <http://doiTbdForThisDocument/> ;
  rdfs:subClassOf rdfs:Literal ;
  rdfs:label "Photographers Reference Number" ;
  dct:description "An identifier used by the University of Washington Libraries to track a photographer or photographers associated with an image." ;
  rdfs:seeAlso <https://github.com/UniverityOfWashingtonLibrariesSchemas/schemasProject/blob/master/dataDictionaries/html/ayp-horizontal-staff.html> .
