# Classes for CONTENTdm metadata

@prefix cdmc: <http://doiTbdForThisDocument/> .
@prefix rdf: <http://www.w3.org/1999/02/22-rdf-syntax-ns#> .
@prefix rdfs:  <http://www.w3.org/2000/01/rdf-schema#> .
@prefix bf: <http://id.loc.gov/ontologies/bibframe/> .

# Classes:
# cdmc:OrderNumber
# cdmc:NegativeNumber
# cdmc:PhotographersReferenceNumber

# TO-DO:
# Add additional value for comment explaining rationale for creating new classes?

cdmc:OrderNumber a rdfs:Class ;
  rdfs:isDefinedBy <http://doiTbdForThisDocument/> ;
  rdfs:subClassOf  bf:Identifier ;
  rdfs:label "Order Number"@en ;
  rdfs:comment "An order number for the item to be used when contacting the University of Washington Libraries Special Collections Reproduction Services."@en .

cdmc:NegativeNumber a rdfs:Class ;
  rdfs:isDefinedBy <http://doiTbdForThisDocument/> ;
  rdfs:subClassOf  bf:Identifier ;
  rdfs:label "Negative Number"@en ;
  rdfs:comment "An identifier used by the University of Washington Libraries Special Collections to track a photographic negative or negatives associated with an image."@en .

cdmc:PhotographersReferenceNumber a rdfs:Class ;
  rdfs:isDefinedBy <http://doiTbdForThisDocument/> ;
  rdfs:subClassOf  bf:Identifier ;
  rdfs:label "Photographers Reference Number"@en ;
  rdfs:comment "An identifier used by the University of Washington Libraries to track a photographer or photographers associated with an image."@en .
